WIP support for C integer types

CN_Lib/CN_Lib.lean
@@ -1,9 +1,167 @@
 namespace CN_Lib
 
+-- CN's represents C integer types as mathematical integers with bounds.
+-- The following bounds are enforced by the ownership predicates defined in CN_Lib_Iris.
+-- Bounds on the unsigned integer types.
+abbrev min_UChar : Int := 0
+abbrev max_UChar : Int := 2 ^ 8 - 1
+-- TODO: what to do for Bool?
+abbrev min_UShort := 0
+abbrev max_UShort := 2 ^ 16 - 1
+abbrev min_UInt : Int := 0
+abbrev max_UInt : Int := 2 ^ 32 - 1
+abbrev min_ULong : Int := 0
+abbrev max_ULong : Int := 2 ^ 64 - 1
+
+-- Bounds on the signed integer types.
+abbrev min_Char : Int := -(2 ^ 7 - 1)
+abbrev max_Char : Int := 2 ^ 7 - 1
+abbrev min_Short : Int := -(2 ^ 15 - 1)
+abbrev max_Short : Int := 2 ^ 15 - 1
+abbrev min_Int : Int := -(2 ^ 31 - 1)
+abbrev max_Int : Int := 2 ^ 31 - 1
+abbrev min_Long : Int := -(2 ^ 63 - 1)
+abbrev max_Long : Int := 2 ^ 63 - 1
+
+--  We roll our own pseudo-bitvectors below because we still have to
+--  reason about ownership of individual Ints sometimes.
+@[simp, reducible]
+def Fin_to_Ints (n : Nat) : Int → (Fin n → Int) :=
+  fun v i => (v % 2 ^(8 * (n - i.toNat))) / (2 ^ (8 * (n - 1 - i.toNat)))
+@[simp, reducible]
+def Ints_to_Fin {n : Nat} (f : Fin n → Int) : Int :=
+  List.foldl
+    (fun acc i => acc + f i * 2 ^ (8 * (n - 1 - i.toNat)))
+    0
+    (List.finRange n)
+
+@[simp, reducible]
+def UShort_bytes (v : Int) : Fin 2 → Int :=
+  Fin_to_Ints 2 v
+
+@[simp, reducible]
+def UInt_bytes (v : Int) : Fin 4 → Int :=
+  Fin_to_Ints 4 v
+
+@[simp, reducible]
+def ULong_bytes (v : Int) : Fin 8 → Int :=
+  Fin_to_Ints 8 v
+
+@[simp, reducible]
+def bytes_UShort (f : Fin 2 → Int) : Int :=
+  Ints_to_Fin f
+
+@[simp, reducible]
+def bytes_UInt (f : Fin 4 → Int) : Int :=
+  Ints_to_Fin f
+
+@[simp, reducible]
+def bytes_ULong (f : Fin 8 → Int) : Int :=
+  Ints_to_Fin f
+
+theorem UShort_idem {v : Int} :
+   min_UShort ≤ v ∧ v ≤ max_UShort
+  → v = bytes_UShort (UShort_bytes v) :=
+by
+  intro ⟨Hv , Hv'⟩
+  simp [List.finRange]; lia
+
+theorem UInt_idem {v : Int} :
+   min_UInt ≤ v ∧ v ≤ max_UInt
+  → v = bytes_UInt (UInt_bytes v) :=
+by
+  intro ⟨Hv , Hv'⟩
+  unfold UInt_bytes Fin_to_Ints bytes_UInt Ints_to_Fin List.finRange
+  simp only [List.ofFn, Fin.foldr, Fin.foldr.loop, List.foldl]
+  simp only [Fin.toNat]
+  lia
+
+theorem ULong_idem {v : Int} :
+   min_ULong ≤ v ∧ v ≤ max_ULong
+  → v = bytes_ULong (ULong_bytes v) :=
+by
+  intro ⟨Hv , Hv'⟩
+  unfold ULong_bytes Fin_to_Ints bytes_ULong Ints_to_Fin List.finRange
+  simp only [List.ofFn, Fin.foldr, Fin.foldr.loop, List.foldl]
+  simp only [Fin.toNat]
+  lia
+
+theorem UShort_eq {v v' : Int} :
+    min_UShort ≤ v ∧ v ≤ max_UShort
+  → min_UShort ≤ v' ∧ v' ≤ max_UShort
+  → UShort_bytes v = UShort_bytes v'
+  → v = v' :=
+by
+  intros Hv Hv' H
+  unfold UShort_bytes at H
+  have HEq : v = bytes_UShort (UShort_bytes v) := by
+    apply UShort_idem; assumption
+  have HEq' : v' = bytes_UShort (UShort_bytes v') := by
+    apply UShort_idem; assumption
+  unfold UShort_bytes at HEq HEq'
+  rw [H] at HEq; symm at HEq'
+  rw [HEq'] at HEq; assumption
+
+theorem UInt_eq {v v' : Int} :
+    min_UInt ≤ v ∧ v ≤ max_UInt
+  → min_UInt ≤ v' ∧ v' ≤ max_UInt
+  → UInt_bytes v = UInt_bytes v'
+  → v = v' :=
+by
+  intros Hv Hv' H
+  unfold UInt_bytes at H
+  have HEq : v = bytes_UInt (UInt_bytes v) := by
+    apply UInt_idem; assumption
+  have HEq' : v' = bytes_UInt (UInt_bytes v') := by
+    apply UInt_idem; assumption
+  unfold UInt_bytes at HEq HEq'
+  rw [H] at HEq; symm at HEq'
+  rw [HEq'] at HEq; assumption
+
+theorem ULong_eq {v v' : Int} :
+    min_ULong ≤ v ∧ v ≤ max_ULong
+  → min_ULong ≤ v' ∧ v' ≤ max_ULong
+  → ULong_bytes v = ULong_bytes v'
+  → v = v' :=
+by
+  intros Hv Hv' H
+  unfold ULong_bytes at H
+  have HEq : v = bytes_ULong (ULong_bytes v) := by
+    apply ULong_idem; assumption
+  have HEq' : v' = bytes_ULong (ULong_bytes v') := by
+    apply ULong_idem; assumption
+  unfold ULong_bytes at HEq HEq'
+  rw [H] at HEq; symm at HEq'
+  rw [HEq'] at HEq; assumption
+
+-- Other stuff
 def wrapI (minInt : Int) (maxInt : Int) x :=
   let delta := ((maxInt - minInt) + 1)
   let r := x % delta
   (if (r <= maxInt) then r else r - delta)
+
+theorem wrapI_within_bounds :
+  ∀ {min max x : Int},
+  (min ≤ 0 ∧ 0 < max) →
+  min ≤ wrapI min max x ∧ wrapI min max x ≤ max :=
+by
+  intro min max x H
+  unfold wrapI
+  let delta := max - min + 1
+  simp; constructor
+  · by_cases h : x % (max - min + 1) ≤ max
+    · simp [h]
+      have hnonneg : 0 ≤ x % (max - min + 1) := by
+        exact Int.emod_nonneg x (by omega)
+      omega
+    · simp [h]; omega
+  · by_cases h : x % (max - min + 1) ≤ max
+    · simp [h]
+    · simp [h]
+      have hd : 0 < max - min + 1 := by omega
+      have hmod : x % (max - min + 1) < max - min + 1 := by
+        exact Int.emod_lt_of_pos x hd
+      omega
 
 theorem dvd_mod_minus (a b c : Int):
   (0 ≤ c) ∧ (c < b) → (b ∣ a - c) → a % b = c :=
@@ -13,22 +171,140 @@ by
   simp [ha, Int.add_mul_emod_self_left, Int.emod_eq_of_lt hc0 hcb]
 
 theorem wrapI_idem:
-  ∀ (minInt maxInt x : Int),
-  (minInt ≤ x ∧ x ≤ maxInt) →
-  (minInt ≤ 0 ∧ 0 < maxInt) →
-  wrapI minInt maxInt x = x :=
+  ∀ {min max x : Int},
+  (min ≤ x ∧ x ≤ max) →
+  (min ≤ 0 ∧ 0 < max) →
+  wrapI min max x = x :=
 by
-  intros minInt maxInt x H1 H2
+  intros min max x H1 H2
   unfold wrapI
-  let delta := ((maxInt - minInt) + 1)
+  let delta := ((max - min) + 1)
   by_cases hx : 0 ≤ x
   · simp
     rw [Int.emod_eq_of_lt]
     omega; exact hx ;omega
   · simp
     rw [dvd_mod_minus _ _ (x + delta)]
-    · by_cases hx' : (x + delta <= maxInt)
+    · by_cases hx' : (x + delta <= max)
       · omega
       · omega
     · omega
     · exists (-1); omega
+
+theorem wrapI_pos_neg_neq :
+  ∀ {max Umax v v' : Int} {_: Umax = 2 * max + 1},
+  0 ≤ v ∧ v ≤ max →
+  -max ≤ v' ∧ v' < 0 →
+  wrapI 0 Umax v ≠ wrapI 0 Umax v' :=
+by
+  intros max Umax v v' inv Hv Hv'
+  unfold wrapI
+  simp [inv, Int.add_assoc]
+  have hvrem : v % (2 * max + 2) = v := by
+    apply Int.emod_eq_of_lt
+    · exact ‹0 ≤ v ∧ v ≤ max›.1
+    · omega
+  have hv'rem : v' % (2 * max + 2) = v' + (2 * max + 2) := by
+    rw [Int.emod_eq_add_self_emod]
+    apply Int.emod_eq_of_lt; omega; omega
+  rw [hvrem, hv'rem]; omega
+
+theorem wrapI_cong_pos :
+  ∀ {max Umax v v' : Int} {_ : 0 ≤ max}
+    {_ : Umax = (2 * max + 1)},
+    0 ≤ v ∧ v ≤ max
+  → 0 ≤ v' ∧ v' ≤ max
+  → wrapI 0 Umax v = wrapI 0 Umax v'
+  → v = v' :=
+by
+  intro max Umax v v' hpos inv ⟨H1, H1'⟩ ⟨H2, H2'⟩ Hwrap
+  have HEq : wrapI 0 Umax v = v := by
+        apply wrapI_idem; lia
+        simp [inv]; lia
+  have HEq' : wrapI 0 Umax v' = v' := by
+    apply wrapI_idem; lia
+    simp [inv]; lia
+  rw [HEq, HEq'] at Hwrap; assumption
+
+theorem wrapI_cong_neg :
+  ∀ {max Umax v v' : Int} {_ : 0 ≤ max}
+    {_ : Umax = (2 * max + 1)},
+    -max ≤ v ∧ v < 0
+  → -max ≤ v' ∧ v' < 0
+  → wrapI 0 Umax v = wrapI 0 Umax v'
+  → v = v' :=
+by
+  intro max Umax v v' hmax hU hv hv' hEq
+  have hmod : 0 < 2 * max + 2 := by omega
+  have hrem : v % (2 * max + 2) < 2 * max + 2 := by
+    exact Int.emod_lt_of_pos v hmod
+  have hrem' : v' % (2 * max + 2) < 2 * max + 2 := by
+    exact Int.emod_lt_of_pos v' hmod
+  have h : v % (2 * max + 2) ≤ 2 * max + 1 := by omega
+  have h' : v' % (2 * max + 2) ≤ 2 * max + 1 := by omega
+  simp [wrapI, hU, Int.add_assoc, h, h'] at hEq
+  have hvrem :
+    v % (2 * max + 2) = v + (2 * max + 2) := by
+    rw [Int.emod_eq_add_self_emod]
+    apply Int.emod_eq_of_lt <;> omega
+  have hvrem' :
+    v' % (2 * max + 2) = v' + (2 * max + 2) := by
+    rw [Int.emod_eq_add_self_emod]
+    apply Int.emod_eq_of_lt <;> omega
+  rw [hvrem, hvrem'] at hEq
+  omega
+
+theorem wrapI_cong :
+  ∀ {max v v' : Int}, 0 ≤ max
+  → -max ≤ v ∧ v ≤ max
+  → -max ≤ v' ∧ v' ≤ max
+  → wrapI 0 (2 * max + 1) v = wrapI 0 (2 * max + 1) v'
+  → v = v' :=
+by
+  intro max v v' hpos ⟨H1, H1'⟩ ⟨H2, H2'⟩ Hwrap
+  by_cases h0 : 0 ≤ v
+  · by_cases h0' : 0 ≤ v'
+    · have h : 0 ≤ v ∧ v ≤ max := by omega
+      have h' : 0 ≤ v' ∧ v' ≤ max := by omega
+      apply wrapI_cong_pos h h' Hwrap;
+      assumption; rfl
+    · exfalso
+      have h : 0 ≤ v ∧ v ≤ max := by omega
+      have h' : -max ≤ v' ∧ v' < 0 := by omega
+      apply wrapI_pos_neg_neq h h' Hwrap; rfl
+  · by_cases h0' : 0 ≤ v'
+    · exfalso
+      have h : -max ≤ v ∧ v < 0 := by omega
+      have h' : 0 ≤ v' ∧ v' ≤ max := by omega
+      apply wrapI_pos_neg_neq h' h Hwrap.symm; rfl
+    · have h : -max ≤ v ∧ v < 0 := by omega
+      have h' : -max ≤ v' ∧ v' < 0 := by omega
+      apply wrapI_cong_neg h h' Hwrap;
+      assumption; rfl
+
+theorem wrapI_Char_cong :
+  min_Char ≤ v ∧ v ≤ max_Char
+  → min_Char ≤ v' ∧ v' ≤ max_Char
+  → wrapI min_UChar max_UChar v = wrapI min_UChar max_UChar v'
+  → v = v' :=
+by
+  intro Hv Hv' Hwrap
+  apply wrapI_cong _ Hv Hv' Hwrap; omega
+
+theorem wrapI_Short_cong :
+  min_Short ≤ v ∧ v ≤ max_Short
+  → min_Short ≤ v' ∧ v' ≤ max_Short
+  → wrapI min_UShort max_UShort v = wrapI min_UShort max_UShort v'
+  → v = v' :=
+by
+  intro Hv Hv' Hwrap
+  apply wrapI_cong _ Hv Hv' Hwrap; omega
+
+theorem wrapI_Int_cong :
+  min_Int ≤ v ∧ v ≤ max_Int
+  → min_Int ≤ v' ∧ v' ≤ max_Int
+  → wrapI min_UInt max_UInt v = wrapI min_UInt max_UInt v'
+  → v = v' :=
+by
+  intro Hv Hv' Hwrap
+  apply wrapI_cong _ Hv Hv' Hwrap; omega
