CN_Lib/CN_Lib_Iris.lean
@@ -5,15 +5,19 @@ import Iris.BI.Lib.GenHeap
 import Iris.Std.GenSetsInstances
 import Iris.ProofMode
 import Std.Data.ExtTreeMap
+import CN_Lib.CN_Lib
+import Lean.Elab
+import Lean
 
-open Iris ProgramLogic Language.Notation Std FromMathlib
+open Lean Elab Tactic Qq
+open Iris ProgramLogic Language.Notation Std FromMathlib BI
 
 namespace CN_Lib
 
 -- Library for things needed by CN lemma exports.
 
 -- 1, Resource algebra for heaps that are maps from integers
---  to integers. Nothing fancy and copied from HeapLang.
+--  to integers.
 
 abbrev myHeapF := fun V => Std.ExtTreeMap Int V compare
 
@@ -32,98 +36,200 @@ class MyHeap (hlc : outParam HasLC) (GF : BundledGFunctors) extends genHeapGS Pt
 variable [MyHeap hlc GF]
 
 
--- 2, Now we add basic CN-style ownership predicates.
+-- 2, CN-style ownership predicates.
+-- Every ownership predicate reduces to ownership of unsigned
+-- bytes and a proof that the value is within bounds for that type.
 
--- Placeholder for int to bytes conversion
-abbrev byte := Int × Int × Int × Int
-def int_to_bytes (v : Int) : byte := sorry
+-- Ownership of unsigned C integer types
+def Owned_UChar (l : Ptr) (v : Int) : IProp GF := iprop%
+    (l ↦ some v) -- Pointsto predicate
+  ∗ ⌜l ≠ 0⌝ -- Pointer is non-null
+  ∗ ⌜ min_UChar ≤ v ∧ v ≤ max_UChar ⌝ -- Value is within bounds
+def Owned_UShort (l : Ptr) (v : Int) : IProp GF :=
+  let bytes := UShort_bytes v
+    iprop% Owned_UChar l (bytes 0)
+  ∗ Owned_UChar (l + 1) (bytes 1)
+  ∗ ⌜ min_UShort ≤ v ∧ v ≤ max_UShort ⌝
+def Owned_UInt (l : Ptr) (v : Int) : IProp GF :=
+  let bytes := UInt_bytes v
+  iprop%
+    ([∗list] i ↦ b ∈ List.ofFn bytes, Owned_UChar (l + i) b)
+  ∗ ⌜ min_UInt ≤ v ∧ v ≤ max_UInt ⌝
+def Owned_ULong (l : Ptr) (v : Int) : IProp GF :=
+  let bytes := ULong_bytes v
+  iprop%
+    ([∗list] i ↦ b ∈ List.ofFn bytes, Owned_UChar (l + i) b)
+  ∗ ⌜ min_ULong ≤ v ∧ v ≤ max_ULong ⌝
 
--- Generic ownership
-def Owned (l : Ptr) (v : Int) : IProp GF := iprop% (l ↦ some v) ∧ ⌜l ≠ 0⌝
-def Block (l : Ptr) : IProp GF := iprop% (l ↦ none) ∧ ⌜l ≠ 0⌝
+-- Ownership of signed C integer types
+def Owned_Char (l : Ptr) (v : Int) : IProp GF :=
+  let byte := wrapI min_UChar max_UChar v
+  iprop%
+    Owned_UChar l byte
+  ∗ ⌜ min_Char ≤ v ∧ v ≤ max_Char ⌝
+def Owned_Short (l : Ptr) (v : Int) : IProp GF :=
+  let bytes := UShort_bytes (wrapI min_UShort max_UShort v)
+  iprop%
+    Owned_UChar l (bytes 0)
+  ∗ Owned_UChar (l + 1) (bytes 1)
+  ∗ ⌜ min_Short ≤ v ∧ v ≤ max_Short ⌝
+def Owned_Int (l : Ptr) (v : Int) : IProp GF :=
+  let bytes := UInt_bytes (wrapI min_UInt max_UInt v)
+  iprop%
+    ([∗list] i ↦ b ∈ List.ofFn bytes, Owned_UChar (l + i) b)
+  ∗ ⌜ min_Int ≤ v ∧ v ≤ max_Int ⌝
+def Owned_Long (l : Ptr) (v : Int) : IProp GF :=
+  let bytes := ULong_bytes (wrapI min_ULong max_ULong v)
+  iprop%
+    ([∗list] i ↦ b ∈ List.ofFn bytes, Owned_UChar (l + i) b)
+  ∗ ⌜ min_Long ≤ v ∧ v ≤ max_Long ⌝
 
--- Ownership of C types
-def Owned_char (l : Ptr) (v : Int) : IProp GF := Owned l v
-def Owned_int (l : Ptr) (v : Int) : IProp GF :=
-  let (b1, b2, b3, b4) := int_to_bytes v
-    iprop% Owned l b1
-    ∗ Owned (l + 1) b2
-    ∗ Owned (l + 2) b3
-    ∗ Owned (l + 3) b4
--- TODO: more C types, e.g. struct, array, etc.
 
 -- 3, Array ownership
 
--- Arrayshift
+def Block (l : Ptr) : IProp GF := iprop% (l ↦ none) ∧ ⌜l ≠ 0⌝
+
 def arrayshift (l : Ptr) (pos : Int) (size : Int) : Ptr := l + pos * size
+
 def padding (l : Ptr) (n : Nat) : IProp GF :=
   match n with
   | 0 => l ↦ none
   | Nat.succ n' => iprop% (Block l ∗ padding (l + 1) n')
 
 
--- 4, Useful lemmas
-
--- Owned pointers can't be null
+-- 4, Pointer non-null theorems
 theorem ptr_nonnull {l : Ptr} {v : Int} :
-  ⊢@{IProp GF} Owned l v → ⌜l ≠ 0⌝ :=
+  ⊢@{IProp GF} Owned_UChar l v → ⌜l ≠ 0⌝ :=
 by
-  unfold Owned
-  iintro ⟨_ , HOwn⟩; iframe
+  unfold Owned_UChar
+  iintro ⟨_ , ⟨HOwn, _⟩⟩; iframe
 
 -- Owned integer pointers can't be null
 theorem ptr_int_nonnull {l : Ptr} {v : Int} :
-  ⊢@{IProp GF} Owned_int l v → ⌜l ≠ 0⌝ :=
+  ⊢@{IProp GF} Owned_Int l v → ⌜l ≠ 0⌝ :=
 by
-  unfold Owned_int Owned
-  iintro ⟨⟨ _ , H⟩ , _⟩; iframe
+  unfold Owned_Int Owned_UChar
+  iintro ⟨H , _⟩
+  simp
+  icases H with ⟨⟨_ , ⟨H , _⟩⟩ , _⟩; iframe
 
--- Two owned pointers must be different
-theorem owned_neq {l l' : Ptr} {v v' : Int} :
-  ⊢@{IProp GF} Owned l v -∗ Owned l' v' -∗ ⌜l ≠ l'⌝ :=
-by
-  unfold Owned
-  iintro ⟨H1 , _⟩ ⟨H2 , _⟩
-  iapply pointsTo_ne $$ H1 H2
+-- TODO: fill these in
 
--- Two owned char pointers must be different
-theorem owned_char_neq {l l' : Ptr} {v v' : Int} :
-  ⊢@{IProp GF} Owned_char l v -∗ Owned_char l' v' -∗ ⌜l ≠ l'⌝ :=
-by
-  unfold Owned_char
-  iintro H1 H2
-  iapply owned_neq $$ H1 H2
+-- 5, Equality theorems for ownership predicates
 
--- Two owned int pointers must be different
-theorem owned_int_neq {l l' : Ptr} {v v' : Int} :
-  ⊢@{IProp GF} Owned_int l v -∗ Owned_int l' v' -∗ ⌜l ≠ l'⌝ :=
+theorem Owned_UChar_eq {l : Ptr} {v v' : Int} :
+  ⊢@{IProp GF} Owned_UChar l v -∗ Owned_UChar l v' -∗ ⌜v = v'⌝ :=
 by
-  unfold Owned_int; simp
-  iintro ⟨H1 , _⟩ ⟨H2 , _⟩
-  iapply owned_neq $$ H1 H2
-
--- Two copies of ownership of the same pointer must have the same value
-theorem owned_eq {l : Ptr} {v v' : Int} :
-  ⊢@{IProp GF} Owned l v -∗ Owned l v' -∗ ⌜v = v'⌝ :=
-by
-  unfold Owned
-  iintro ⟨H1 , _⟩ ⟨H2 , _⟩
+  unfold Owned_UChar min_UChar max_UChar
+  iintro ⟨H1 , ⟨_ , ⟨%h1, %h1'⟩⟩⟩ ⟨H2 , ⟨_ , ⟨%h2 , %h2'⟩⟩⟩
   ihave %H := pointsTo_agree $$ [$]
-  ipureintro; injection H; omega
+  ipureintro; injection H with val_eq; lia
 
--- Two copies of ownership of the same char pointer must have the same value
-theorem owned_char_eq {l : Ptr} {v v' : Int} :
-  ⊢@{IProp GF} Owned_char l v -∗ Owned_char l v' -∗ ⌜v = v'⌝ :=
+theorem Owned_Char_eq {l : Ptr} {v v' : Int} :
+  ⊢@{IProp GF} Owned_Char l v -∗ Owned_Char l v' -∗ ⌜v = v'⌝ :=
 by
-  unfold Owned_char
-  iintro H1 H2
-  iapply owned_eq $$ H1 H2
+  unfold Owned_Char min_Char max_Char
+  iintro ⟨H1 , %H2⟩ ⟨H3 , %H4⟩
+  ihave %HEq := Owned_UChar_eq $$ H1 H3
+  ipureintro
+  apply wrapI_Char_cong H2 H4 HEq
 
--- Two copies of ownership of the same int pointer must have the same value
-theorem owned_int_eq {l : Ptr} {v v' : Int} :
-  ⊢@{IProp GF} Owned_int l v -∗ Owned_int l v' -∗ ⌜v = v'⌝ :=
+theorem Owned_UShort_eq {l : Ptr} {v v' : Int} :
+  ⊢@{IProp GF} Owned_UShort l v -∗ Owned_UShort l v' -∗ ⌜v = v'⌝ :=
 by
-  sorry
--- TODO: Omitted until int_to_bytes is implemented
+  unfold Owned_UShort min_UShort max_UShort
+  iintro ⟨H1 , ⟨H2 , ⟨%H⟩⟩⟩ ⟨H5 , ⟨H6 , ⟨%H'⟩⟩⟩
+  ihave %HEq := Owned_UChar_eq $$ H1 H5
+  ihave %HEq' := Owned_UChar_eq $$ H2 H6
+  ipureintro
+  have Hbytes : UShort_bytes v = UShort_bytes v' := by
+    funext i
+    repeat refine Fin.lastCases ?_ ?_ i; lia; intro i
+    apply Fin.elim0; assumption
+  have H := UShort_eq H H' Hbytes
+  assumption
 
-end CN_Lib
+theorem Owned_Short_eq {l : Ptr} {v v' : Int} :
+  ⊢@{IProp GF} Owned_Short l v -∗ Owned_Short l v' -∗ ⌜v = v'⌝ :=
+by
+  unfold Owned_Short
+  iintro ⟨H1 , ⟨H2 , %H⟩⟩ ⟨H3 , ⟨H4 , %H'⟩⟩
+  ihave %HEq := Owned_UChar_eq $$ H1 H3
+  ihave %HEq' := Owned_UChar_eq $$ H2 H4
+  ipureintro
+  have Hbytes : UShort_bytes (wrapI min_UShort max_UShort v) = UShort_bytes (wrapI min_UShort max_UShort v') := by
+    funext i
+    repeat refine Fin.lastCases ?_ ?_ i; lia; intro i
+    apply Fin.elim0; assumption
+  have Hv := wrapI_within_bounds (x := v) (min := min_UShort) (max := max_UShort) (by lia)
+  have Hv' := wrapI_within_bounds (x := v') (min := min_UShort) (max := max_UShort) (by lia)
+  have H1 := UShort_eq Hv Hv' Hbytes
+  apply wrapI_Short_cong H H' H1
+
+theorem Owned_UInt_eq {l : Ptr} {v v' : Int} :
+  ⊢@{IProp GF} Owned_UInt l v -∗ Owned_UInt l v' -∗ ⌜v = v'⌝ :=
+by
+  unfold Owned_UInt
+  iintro ⟨HOwn, %H⟩ ⟨HOwn', %H'⟩
+  simp [-UInt_bytes]
+  icases HOwn with ⟨H1 , ⟨H2 , ⟨H3 , ⟨H4 , _⟩⟩⟩⟩
+  icases HOwn' with ⟨H1' , ⟨H2' , ⟨H3' , ⟨H4' , _⟩⟩⟩⟩
+  ihave %H1 := Owned_UChar_eq $$ H1 H1'
+  ihave %H2 := Owned_UChar_eq $$ H2 H2'
+  ihave %H3 := Owned_UChar_eq $$ H3 H3'
+  ihave %H4 := Owned_UChar_eq $$ H4 H4'
+  ipureintro
+  have Hbytes : UInt_bytes v = UInt_bytes v' := by
+    funext i
+    repeat refine Fin.lastCases ?_ ?_ i; lia; intro i
+    apply Fin.elim0; assumption
+  have H1 := UInt_eq H H' Hbytes
+  assumption
+
+theorem Owned_Int_eq {l : Ptr} {v v' : Int} :
+  ⊢@{IProp GF} Owned_Int l v -∗ Owned_Int l v' -∗ ⌜v = v'⌝ :=
+by
+  unfold Owned_Int
+  iintro ⟨HOwn, %H⟩ ⟨HOwn', %H'⟩
+  simp [-UInt_bytes]
+  icases HOwn with ⟨H1 , ⟨H2 , ⟨H3 , ⟨H4 , _⟩⟩⟩⟩
+  icases HOwn' with ⟨H1' , ⟨H2' , ⟨H3' , ⟨H4' , _⟩⟩⟩⟩
+  ihave %H1 := Owned_UChar_eq $$ H1 H1'
+  ihave %H2 := Owned_UChar_eq $$ H2 H2'
+  ihave %H3 := Owned_UChar_eq $$ H3 H3'
+  ihave %H4 := Owned_UChar_eq $$ H4 H4'
+  ipureintro
+  have Hbytes : UInt_bytes (wrapI min_UInt max_UInt v) = UInt_bytes (wrapI min_UInt max_UInt v') := by
+    funext i
+    repeat refine Fin.lastCases ?_ ?_ i; lia; intro i
+    apply Fin.elim0; assumption
+  have Hv := wrapI_within_bounds (x := v) (min := min_UInt) (max := max_UInt) (by lia)
+  have Hv' := wrapI_within_bounds (x := v') (min := min_UInt) (max := max_UInt) (by lia)
+  have H1 := UInt_eq Hv Hv' Hbytes
+  apply wrapI_Int_cong H H' H1
+
+theorem Owned_ULong_eq {l : Ptr} {v v' : Int} :
+  ⊢@{IProp GF} Owned_ULong l v -∗ Owned_ULong l v' -∗ ⌜v = v'⌝ :=
+by
+  unfold Owned_ULong
+  iintro ⟨HOwn, %H⟩ ⟨HOwn', %H'⟩
+  simp [-ULong_bytes]
+  icases HOwn with ⟨H1 , ⟨H2 , ⟨H3 , ⟨H4 , HOwn⟩⟩⟩⟩
+  icases HOwn with ⟨H5 , ⟨H6 , ⟨H7 , ⟨H8 , _⟩⟩⟩⟩
+  icases HOwn' with ⟨H1' , ⟨H2' , ⟨H3' , ⟨H4' , HOwn'⟩⟩⟩⟩
+  icases HOwn' with ⟨H5' , ⟨H6' , ⟨H7' , ⟨H8' , _⟩⟩⟩⟩
+  ihave %H1 := Owned_UChar_eq $$ H1 H1'
+  ihave %H2 := Owned_UChar_eq $$ H2 H2'
+  ihave %H3 := Owned_UChar_eq $$ H3 H3'
+  ihave %H4 := Owned_UChar_eq $$ H4 H4'
+  ihave %H5 := Owned_UChar_eq $$ H5 H5'
+  ihave %H6 := Owned_UChar_eq $$ H6 H6'
+  ihave %H7 := Owned_UChar_eq $$ H7 H7'
+  ihave %H8 := Owned_UChar_eq $$ H8 H8'
+  ipureintro
+  have Hbytes : ULong_bytes v = ULong_bytes v' := by
+    funext i
+    repeat refine Fin.lastCases ?_ ?_ i; lia; intro i
+    apply Fin.elim0; assumption
+  have H1 := ULong_eq H H' Hbytes
+  assumption
